src/dafny/beacon/statetransition/EpochProcessing.dfy
@@ -17,13 +17,14 @@ include "../../ssz/Constants.dfy"
 include "../attestations/AttestationsTypes.dfy"
 include "../Helpers.dfy"
 include "../attestations/AttestationsHelpers.dfy"
+include "../validators/ValidatorHelpers.dfy"
 include "EpochProcessing.s.dfy"
 include "ProcessOperations.s.dfy"
 include "../../utils/Eth2Types.dfy"
 include "../../utils/MathHelpers.dfy"
 
 /**
- * State transition function for the Beacon Chain.
+ * Epoch processing and related functions for the Beacon Chain.
  */
 module EpochProcessing {
     
@@ -32,6 +33,7 @@ module EpochProcessing {
     import opened Constants
     import opened BeaconChainTypes
     import opened AttestationsTypes
+    import opened ValidatorHelpers
     import opened BeaconHelpers
     import opened AttestationsHelpers
     import opened EpochProcessingSpec
@@ -39,39 +41,32 @@ module EpochProcessing {
     import opened Eth2Types
     import opened MathHelpers
 
-// # Attestations
-//     previous_epoch_attestations: List[PendingAttestation, MAX_ATTESTATIONS * SLOTS_PER_EPOCH]
-//     current_epoch_attestations: List[PendingAttestation, MAX_ATTESTATIONS * SLOTS_PER_EPOCH]
-//     # Finality
-//     justification_bits: Bitvector[JUSTIFICATION_BITS_LENGTH]  # Bit set for every recent justified epoch
-//     previous_justified_checkpoint: Checkpoint  # Previous epoch snapshot
-//     current_justified_checkpoint: Checkpoint
-//     finalized_checkpoint: Checkpoint
-
-
     /**
      *  At epoch boundaries, update justifications, rewards, penalities,
-     *  resgistry, slashing, and final updates.
+     *  resgistry, slashing, and final updates, etc.
      *
      *  @param  s   A beacon state.
-     *  @returns    
-     *  @note       ?? Mention any simplifcations
+     *  @returns    A new state resulting from the processing of the epoch components.
+     *  @note       The process_effective_balance_updates component has been simplified.
      */
     method process_epoch(s: BeaconState) returns (s' : BeaconState) 
         //  Make sure s.slot does not overflow
         requires s.slot as nat + 1 < 0x10000000000000000 as nat
         //  And we should only execute this method when:
         requires (s.slot + 1) % SLOTS_PER_EPOCH == 0
-
         requires |s.validators| == |s.balances|
-        //requires if get_current_epoch(s) > GENESIS_EPOCH + 1 then  get_previous_epoch(s) >= s.finalised_checkpoint.epoch else true
-        //requires if get_current_epoch(s) != GENESIS_EPOCH then  EFFECTIVE_BALANCE_INCREMENT <= get_total_active_balance(s) else true
-        //requires if get_current_epoch(s) != GENESIS_EPOCH then  1 <= get_previous_epoch(s) else true // <= get_current_epoch(s)
-        requires forall a :: a in s.previous_epoch_attestations ==> a.data.index < get_committee_count_per_slot(s, compute_epoch_at_slot(a.data.slot)) <= TWO_UP_6 
-        requires forall a :: a in s.previous_epoch_attestations ==> TWO_UP_5 as nat <= |get_active_validator_indices(s.validators, compute_epoch_at_slot(a.data.slot))| <= TWO_UP_11 as nat * TWO_UP_11 as nat 
-        requires forall a :: a in s.previous_epoch_attestations ==> 0 < |get_beacon_committee(s, a.data.slot, a.data.index)| == |a.aggregation_bits| <= MAX_VALIDATORS_PER_COMMITTEE as nat
+        requires forall a :: a in s.previous_epoch_attestations 
+                    ==> a.data.index 
+                        < get_committee_count_per_slot(s, compute_epoch_at_slot(a.data.slot)) 
+                        <= TWO_UP_6 
+        requires forall a :: a in s.previous_epoch_attestations 
+                    ==> TWO_UP_5 as nat 
+                        <= |get_active_validator_indices(s.validators, compute_epoch_at_slot(a.data.slot))| 
+                        <= TWO_UP_11 as nat * TWO_UP_11 as nat 
+        requires forall a :: a in s.previous_epoch_attestations 
+                    ==> 0 < |get_beacon_committee(s, a.data.slot, a.data.index)| 
+                        == |a.aggregation_bits| <= MAX_VALIDATORS_PER_COMMITTEE as nat
       
-        // /** Leaves some fields unchanged. */
         ensures s'.slot == s.slot
         ensures s'.eth1_deposit_index == s.eth1_deposit_index
         ensures |s'.validators| == |s'.balances|
@@ -82,62 +77,144 @@ module EpochProcessing {
 
         assert s' == updateFinalisedCheckpoint(updateJustification(s), s);
         assert s' == updateJustificationAndFinalisation(s);
-        ghost var s1 := s';
-
         assert s'.previous_epoch_attestations == s.previous_epoch_attestations;
         assert s'.validators == s.validators;
-        
-        assert forall a :: a in s'.previous_epoch_attestations ==> a.data.index < get_committee_count_per_slot(s', compute_epoch_at_slot(a.data.slot)) <= TWO_UP_6 ;
-        assert forall a :: a in s'.previous_epoch_attestations ==> TWO_UP_5 as nat <= |get_active_validator_indices(s'.validators, compute_epoch_at_slot(a.data.slot))| <= TWO_UP_11 as nat * TWO_UP_11 as nat ;
-        assert forall a :: a in s'.previous_epoch_attestations ==> 0 < |get_beacon_committee(s', a.data.slot, a.data.index)| == |a.aggregation_bits| <= MAX_VALIDATORS_PER_COMMITTEE as nat;
+        assert forall a :: a in s'.previous_epoch_attestations 
+                ==> a.data.index < get_committee_count_per_slot(s', compute_epoch_at_slot(a.data.slot)) 
+                    <= TWO_UP_6 ;
+        assert forall a :: a in s'.previous_epoch_attestations 
+                ==> TWO_UP_5 as nat 
+                    <= |get_active_validator_indices(s'.validators, compute_epoch_at_slot(a.data.slot))| 
+                    <= TWO_UP_11 as nat * TWO_UP_11 as nat ;
+        assert forall a :: a in s'.previous_epoch_attestations 
+                ==> 0 < |get_beacon_committee(s', a.data.slot, a.data.index)|
+                    == |a.aggregation_bits| <= MAX_VALIDATORS_PER_COMMITTEE as nat;
 
         s' := process_rewards_and_penalties(s');
 
         assert s' == updateRAndP(updateJustificationAndFinalisation(s));
-        
-        // process_registry_updates(state)
-
+    
         assert |s'.validators| == |s'.balances| == |s.validators|;
         s' := process_slashings(s');
-        assert s' == updateSlashings(updateRAndP(updateJustificationAndFinalisation(s)));
+        assert s' == updateSlashings(
+                        updateRAndP(
+                                updateJustificationAndFinalisation(s)
+                        )
+                     );
 
         s' := process_eth1_data_reset(s');
-        assert s' == updateEth1DataReset(updateSlashings(updateRAndP(updateJustificationAndFinalisation(s))));
+        assert s' == updateEth1DataReset(
+                        updateSlashings(
+                            updateRAndP(
+                                updateJustificationAndFinalisation(s)
+                            )
+                        )
+                     );
 
         assert |s'.validators| == |s'.balances| == |s.validators|;
         s' := process_effective_balance_updates(s');
-        assert s' == updateEffectiveBalance(updateEth1DataReset(updateSlashings(updateRAndP(updateJustificationAndFinalisation(s)))));
+        assert s' == updateEffectiveBalance(
+                        updateEth1DataReset(
+                            updateSlashings(
+                                updateRAndP(
+                                    updateJustificationAndFinalisation(s)
+                                )
+                            )
+                        )
+                     );
 
         s' := process_slashings_reset(s');
-        assert s' == updateSlashingsReset(updateEffectiveBalance(updateEth1DataReset(updateSlashings(updateRAndP(updateJustificationAndFinalisation(s))))));
+        assert s' == updateSlashingsReset(
+                        updateEffectiveBalance(
+                            updateEth1DataReset(
+                                updateSlashings(
+                                    updateRAndP(
+                                        updateJustificationAndFinalisation(s)
+                                    )
+                                )
+                            )
+                        )
+                     );
 
         s' := process_randao_mixes_reset(s');
-        assert s' == updateRandaoMixes(updateSlashingsReset(updateEffectiveBalance(updateEth1DataReset(updateSlashings(updateRAndP(updateJustificationAndFinalisation(s)))))));
+        assert s' == updateRandaoMixes(
+                        updateSlashingsReset(  
+                            updateEffectiveBalance(
+                                updateEth1DataReset(
+                                    updateSlashings(
+                                        updateRAndP(
+                                            updateJustificationAndFinalisation(s)
+                                        )
+                                    )
+                                )
+                            )
+                        )
+                     );
 
         s' := process_historical_roots_update(s');
-        assert s' == updateHistoricalRoots(updateRandaoMixes(updateSlashingsReset(updateEffectiveBalance(updateEth1DataReset(updateSlashings(updateRAndP(updateJustificationAndFinalisation(s))))))));
+        assert s' == updateHistoricalRoots(
+                        updateRandaoMixes( 
+                            updateSlashingsReset(
+                                updateEffectiveBalance(
+                                    updateEth1DataReset(
+                                        updateSlashings(
+                                            updateRAndP(
+                                                updateJustificationAndFinalisation(s)
+                                            )
+                                        )
+                                    )
+                                )
+                            )
+                        )
+                     );
 
         s' := process_participation_record_updates(s');
-        assert s' == updateParticipationRecords(updateHistoricalRoots(updateRandaoMixes(updateSlashingsReset(updateEffectiveBalance(updateEth1DataReset(updateSlashings(updateRAndP(updateJustificationAndFinalisation(s)))))))));
+        assert s' == updateParticipationRecords(
+                        updateHistoricalRoots(
+                            updateRandaoMixes(
+                                updateSlashingsReset(
+                                    updateEffectiveBalance(
+                                        updateEth1DataReset(
+                                            updateSlashings(
+                                                updateRAndP(
+                                                    updateJustificationAndFinalisation(s)
+                                                )
+                                            )
+                                        )
+                                    )
+                                )
+                            )
+                        )
+                     );
 
-        //      s' := process_final_updates(s');
-        // assert(s' == finalUpdates(s2));
-        // assume(s' == forwardStateToSlot(s, s.slot));
-        // assume(s' == resolveStateRoot(s));
         assert s' == updateEpoch(s);
         return s';
     }
     
-    /* */
+    /** 
+     *  Process rewards and penalties.
+     *  
+     *  @param  s   A state.
+     *  @returns    The state obtained after applying the epoch rewards and penalties.
+     *
+     *  @note       This function uses assume statements as a simplification to ensure
+     *              that balance overflows don't occur. To remove these assume statements
+     *              a strategy similar to that applied within the deposit processing
+     *              could be applied.
+     */
     method process_rewards_and_penalties(s: BeaconState)  returns (s' : BeaconState)
         requires |s.validators| == |s.balances|
-        //requires if get_current_epoch(s) > GENESIS_EPOCH + 1 then  get_previous_epoch(s) >= s.finalised_checkpoint.epoch else true
-        //requires if get_current_epoch(s) != GENESIS_EPOCH then  EFFECTIVE_BALANCE_INCREMENT <= get_total_active_balance(s) else true
-       // requires if get_current_epoch(s) != GENESIS_EPOCH then  1 <= get_previous_epoch(s) else true // <= get_current_epoch(s)
-
-        requires forall a :: a in s.previous_epoch_attestations ==> a.data.index < get_committee_count_per_slot(s, compute_epoch_at_slot(a.data.slot)) <= TWO_UP_6 
-        requires forall a :: a in s.previous_epoch_attestations ==> TWO_UP_5 as nat <= |get_active_validator_indices(s.validators, compute_epoch_at_slot(a.data.slot))| <= TWO_UP_11 as nat * TWO_UP_11 as nat 
-        requires forall a :: a in s.previous_epoch_attestations ==> 0 < |get_beacon_committee(s, a.data.slot, a.data.index)| == |a.aggregation_bits| <= MAX_VALIDATORS_PER_COMMITTEE as nat 
+        requires forall a :: a in s.previous_epoch_attestations 
+                    ==> a.data.index < get_committee_count_per_slot(s, compute_epoch_at_slot(a.data.slot)) 
+                        <= TWO_UP_6 
+        requires forall a :: a in s.previous_epoch_attestations 
+                    ==> TWO_UP_5 as nat 
+                        <= |get_active_validator_indices(s.validators, compute_epoch_at_slot(a.data.slot))| 
+                        <= TWO_UP_11 as nat * TWO_UP_11 as nat 
+        requires forall a :: a in s.previous_epoch_attestations 
+                    ==> 0 
+                        < |get_beacon_committee(s, a.data.slot, a.data.index)| == |a.aggregation_bits| 
+                        <= MAX_VALIDATORS_PER_COMMITTEE as nat 
         
         ensures s' == updateRAndP(s)
     {
@@ -150,377 +227,139 @@ module EpochProcessing {
         assume get_previous_epoch(s) >= s.finalised_checkpoint.epoch;
         assert EFFECTIVE_BALANCE_INCREMENT <= get_total_active_balance_full(s); 
         assert 1 <= get_previous_epoch(s);
-        //assume integer_square_root(get_total_active_balance(s)) > 1;
         var (rewards, penalties) := get_attestation_deltas(s');
-        
         var i := 0;
-
         
         assert s' == updateRewardsAndPenalties(s, rewards[..i], penalties[..i]);
-        assume forall v :: 0 <= v < |rewards| ==> s.balances[v] as nat + rewards[v] as nat < 0x10000000000000000;
+        // assume statements are used throughout to prevent overflows 
+        assume forall v :: 0 <= v < |rewards| 
+                ==> s.balances[v] as nat + rewards[v] as nat < 0x10000000000000000;
         
-
-        while i < |s'.validators| //for index in range(len(state.validators)):
+        while i < |s'.validators| 
             invariant i <= |rewards| == |penalties|
-            invariant |rewards| == |penalties| == |s.validators| == |s.balances| == |s'.validators| == |s'.balances|
+            invariant |rewards| 
+                        == |penalties| 
+                        == |s.validators| 
+                        == |s.balances| 
+                        == |s'.validators| 
+                        == |s'.balances|
             invariant |rewards[..i]| == |penalties[..i]| <= |s.validators| == |s.balances|
-            //invariant forall v :: i <= v < |s.balances| ==> s'.balances[v] == s.balances[v]
-            //invariant forall v :: 0 <= v < i ==> s'.balances[v] == if s.balances[v] + rewards[v] > penalties[v] then s.balances[v] + rewards[v] - penalties[v] else 0 as Gwei;
-            //invariant forall v :: 0 <= v < i ==> s'.balances[v] == updateRewardsAndPenalties(s, rewards[..i], penalties[..i]).balances[v];
-            //invariant forall v :: i <= v < |s.balances| ==> s'.balances[v] == s.balances[v] == updateRewardsAndPenalties(s, rewards[..i], penalties[..i]).balances[v];
-            //invariant forall v :: 0 <= v < |s.balances| ==> s'.balances[v] == updateRewardsAndPenalties(s, rewards[..i], penalties[..i]).balances[v];
-            //invariant forall v :: 0 <= v < |s.validators| ==> s'.validators[v] == updateRewardsAndPenalties(s, rewards[..i], penalties[..i]).validators[v];
             invariant i == |rewards[..i]|
             invariant s' == updateRewardsAndPenalties(s, rewards[..i], penalties[..i])
-            //invariant s' == updateRewardsAndPenaltiesWrapper(s)
         {
             assert i < |rewards|;
             assert i < |s'.balances|;
-            //assume s'.balances[i] as nat + rewards[i] as nat < 0x10000000000000000;
-            
             s' := increase_balance(s', i as ValidatorIndex, rewards[i]);
             s' := decrease_balance(s', i as ValidatorIndex, penalties[i]);
-            assert s'.balances[i] == if s.balances[i] + rewards[i] > penalties[i] then s.balances[i] + rewards[i] - penalties[i] else 0 as Gwei;
-            assert forall v :: 0 <= v <= i ==> s'.balances[v] == if s.balances[v] + rewards[v] > penalties[v] then s.balances[v] + rewards[v] - penalties[v] else 0 as Gwei;
+            assert s'.balances[i] == if s.balances[i] + rewards[i] > penalties[i] 
+                                        then s.balances[i] + rewards[i] - penalties[i] 
+                                        else 0 as Gwei;
+            assert forall v :: 0 <= v <= i 
+                    ==> s'.balances[v] == if s.balances[v] + rewards[v] > penalties[v] 
+                                            then s.balances[v] + rewards[v] - penalties[v] 
+                                            else 0 as Gwei;
             i := i + 1;
         } 
         assert rewards[..i] == rewards;
         assert penalties[..i] == penalties;
         assert s' == updateRewardsAndPenalties(s, rewards, penalties);
         assert s' == updateRAndP(s);
-
     }
 
-    // function updateRegistry(s: BeaconState): BeaconState
-    //     requires |s.validators| == |s.balances|
-    //     //ensures updateRegistry(s) == updateEligibilityAndEjectionsHelper(s, |s.validators|)
-    
-
-    function updateEligibility(s: BeaconState): BeaconState
-        requires |s.validators| == |s.balances|
-        ensures updateEligibility(s) == updateEligibilityHelper(s, |s.validators|)
-    {
-        updateEligibilityHelper(s, |s.validators|)
-    }
-
-    function updateEligibilityHelper(s: BeaconState, len: nat): BeaconState
-        requires len <= |s.validators| == |s.balances|
-        ensures |updateEligibilityHelper(s, len).validators| == |s.validators|
-        ensures updateEligibilityHelper(s, len) == s.(validators := updateEligibilityHelper(s, len).validators)
-        ensures forall v :: len <= v < |s.validators| ==> updateEligibilityHelper(s, len).validators[v] == s.validators[v]
-        ensures forall v :: 0 <= v < len ==> 
-            updateEligibilityHelper(s, len).validators[v] == 
-                    if is_eligible_for_activation_queue(s.validators[v])
-                        then s.(validators := s.validators[v := s.validators[v].(activation_eligibility_epoch := get_current_epoch(s) + 1)]).validators[v]
-                        else s.validators[v]
-        decreases len
-    {
-        if len == 0 then s
-        else
-            var i := len -1;
-            assert i < |s.validators|;
-            var s1 := if is_eligible_for_activation_queue(s.validators[i])
-                    then s.(validators := s.validators[i := s.validators[i].(activation_eligibility_epoch := get_current_epoch(s) + 1)])
-                    else s;
-            assert s1.validators[i].activation_eligibility_epoch == if is_eligible_for_activation_queue(s.validators[i]) then get_current_epoch(s) + 1 
-                                                                    else s.validators[i].activation_eligibility_epoch;
-            
-            assert |s1.balances| == |s1.validators| == |s.validators|; 
-            assert forall v :: len <= v < |s.validators| ==> s1.validators[v] == s.validators[v];
-        
-            updateEligibilityHelper(s1, len-1)
-    }
-
-    function updateEjections(s: BeaconState): BeaconState
-        requires |s.validators| == |s.balances|
-        ensures updateEjections(s) == updateEjectionsHelper(s, |s.validators|)
-    {
-        updateEjectionsHelper(s, |s.validators|)
-    }
-
-    function updateEjectionsHelper(s: BeaconState, len: nat): BeaconState
-        requires len <= |s.validators| == |s.balances|
-        ensures updateEjectionsHelper(s, len) == s.(validators := updateEjectionsHelper(s, len).validators)
-
-        ensures |updateEjectionsHelper(s, len).validators| == |s.validators|
-        ensures updateEjectionsHelper(s, len) == s.(validators := updateEjectionsHelper(s, len).validators)
-        ensures forall v :: len <= v < |s.validators| ==> updateEjectionsHelper(s, len).validators[v] == s.validators[v]
-        ensures forall v :: 0 <= v < len ==> 
-            // var new_val := if (is_active_validator(s.validators[v],  get_current_epoch(s)) && s.validators[v].effective_balance <= EJECTION_BALANCE )
-            //             then initiate_validator_exit(s, v as ValidatorIndex).validators[v]
-            //             else s.validators[v];
-            updateEjectionsHelper(s, len).validators[v] == if (is_active_validator(s.validators[v],  get_current_epoch(s)) && s.validators[v].effective_balance <= EJECTION_BALANCE )
-                        then initiate_validator_exit(s, v as ValidatorIndex).validators[v]
-                        else s.validators[v]
-
-        decreases len
-    // {
-    //     if len == 0 then s
-    //     else
-    //         var i := len -1;
-    //         assert i < |s.validators|;
-    //         var s1 := if (is_active_validator(s.validators[i],  get_current_epoch(s)) && s.validators[i].effective_balance <= EJECTION_BALANCE )
-    //             // initiate_validator_exit(state, ValidatorIndex(index))
-    //                 then initiate_validator_exit(s, i as ValidatorIndex)
-    //                 else s;
-    //         assert s1.validators[i] == if (is_active_validator(s.validators[i],  get_current_epoch(s)) && s.validators[i].effective_balance <= EJECTION_BALANCE )
-    //                                         then initiate_validator_exit(s, i as ValidatorIndex).validators[i]
-    //                                         else s.validators[i];
-            
-    //         assert |s1.balances| == |s1.validators| == |s.validators|; 
-    //         assert forall v :: 0 <= v < |s1.balances|  ==> s1.balances[v] == s.balances[v];
-    //         assert forall v :: i < v < |s.validators| ==> s1.validators[v] == s.validators[v];
-    //         assert forall v :: 0 <= v < i ==> s1.validators[v] == s.validators[v];
-    //         updateEjectionsHelper(s1, len-1)
-    // }
-
-    // /** */
-    // method process_registry_updates(s: BeaconState)  returns (s' : BeaconState)
-    //     requires |s.validators| == |s.balances|
-    //     //ensures s' == updateRegistry(s)
-    // {
-    //     //  Process activation eligibility and ejections
-    //     s' := s;
-    //     var i := 0;
-    //     assert s' == updateEligibilityHelper(s', i);
-
-    //     while i < |s'.validators|
-    //         invariant  |s.validators| == |s.balances| ==|s'.balances| == |s'.validators|
-    //         invariant i <= |s'.validators| == |s'.balances| 
-    //         invariant forall v :: 0 <= v < |s.balances| ==> s'.balances[v] ==  s.balances[v]
-    //         invariant forall v :: i <= v < |s.validators| ==> s'.validators[v] ==  s.validators[v]
-            
-    //         invariant s' == s.(validators := s'.validators)
-    //         invariant get_current_epoch(s') == get_current_epoch(s)
-
-    //         invariant forall v :: 0 <= v < i ==> 
-    //             updateEligibilityHelper(s, i).validators[v] == 
-    //                     if is_eligible_for_activation_queue(s.validators[v])
-    //                         then s.(validators := s.validators[v := s.validators[v].(activation_eligibility_epoch := get_current_epoch(s) + 1)]).validators[v]
-    //                         else s.validators[v]
-
-    //         invariant s' == updateEligibilityHelper(s', i)
-    //     {
-    //         assert s'.validators[i] == s.validators[i];
-    //         // is_eligible_for_activation_queue:  v.activation_eligibility_epoch == FAR_FUTURE_EPOCH && v.effective_balance == MAX_EFFECTIVE_BALANCE
-    //         if is_eligible_for_activation_queue(s.validators[i]) {
-    //             //s'.validator[i].activation_eligibility_epoch := get_current_epoch(s') + 1;
-    //             s' := s'.(validators := s'.validators[i := s'.validators[i].(activation_eligibility_epoch := get_current_epoch(s) + 1)]);   
-    //         }
-    //         assert s'.validators[i].activation_eligibility_epoch == if is_eligible_for_activation_queue(s.validators[i]) then get_current_epoch(s) + 1 
-    //                                                                 else s.validators[i].activation_eligibility_epoch;
-            
-    //         i := i + 1;
-            
-    //     }
-    //     assert s' == updateEligibilityHelper(s', i);
-    //     var s1 := s';
-
-    //     // Process ejections
-    //     var j := 0;
-    //     assert s' == updateEjectionsHelper(s1, j);
-    //     while j < |s'.validators|
-    //         invariant  |s1.validators| == |s1.balances| ==|s'.balances| == |s'.validators|
-    //         invariant i <= |s'.validators| == |s'.balances| 
-    //         invariant forall v :: 0 <= v < |s.balances| ==> s'.balances[v] ==  s.balances[v]
-    //         invariant forall v :: j <= v < |s.validators| ==> s'.validators[v] ==  s.validators[v]
-            
-    //         invariant s' == s.(validators := s'.validators)
-    //         invariant get_current_epoch(s') == get_current_epoch(s)
-
-    //         // invariant forall v :: 0 <= v < j ==> 
-    //         //     updateEjectionsHelper(s, j).validators[v] == 
-    //         //             if (is_active_validator(s.validators[j],  get_current_epoch(s)) && s.validators[j].effective_balance <= EJECTION_BALANCE )
-    //         //                then initiate_validator_exit(s, v as ValidatorIndex).validators[v]
-    //         //                 else s.validators[v]
-
-    //         // invariant s' == updateEjectionsHelper(s', j)
-    //     {
-    //         assert s'.validators[j] == s.validators[j];
-    //         if (is_active_validator(s.validators[j],  get_current_epoch(s)) && s.validators[j].effective_balance <= EJECTION_BALANCE ) {
-    //             s' := initiate_validator_exit(s', j as ValidatorIndex);   
-    //         }
-    //         assert s'.validators[i].activation_eligibility_epoch == if is_eligible_for_activation_queue(s.validators[i]) then get_current_epoch(s) + 1 
-    //                                                                 else s.validators[i].activation_eligibility_epoch;
-            
-    //         j := j + 1;
-            
-    //     }
-    //     assert s' == updateEjectionsHelper(s', j);
-
-    //     // while i < |s'.validators|
-    //     //     invariant  |s.validators| == |s.balances| ==|s'.balances| == |s'.validators|
-    //     //     invariant i <= |s'.validators| == |s'.balances| 
-    //     //     invariant forall v :: 0 <= v < |s.balances| ==> s'.balances[v] ==  s.balances[v]
-    //     //     invariant forall v :: i <= v < |s.validators| ==> s'.validators[v] ==  s.validators[v]
-            
-    //     //     invariant s' == s.(validators := s'.validators)
-    //     //     invariant get_current_epoch(s') == get_current_epoch(s)
-    //     //     //invariant s' == updateEligibilityAndEjectionsHelper(s', i)
-    //     // {
-    //     //     assert s'.validators[i] == s.validators[i];
-    //     //     // is_eligible_for_activation_queue:  v.activation_eligibility_epoch == FAR_FUTURE_EPOCH && v.effective_balance == MAX_EFFECTIVE_BALANCE
-    //     //     if is_eligible_for_activation_queue(s.validators[i]) {
-    //     //         //s'.validator[i].activation_eligibility_epoch := get_current_epoch(s') + 1;
-    //     //         s' := s'.(validators := s'.validators[i := s'.validators[i].(activation_eligibility_epoch := get_current_epoch(s) + 1)]);   
-    //     //     }
-    //     //     assert s'.validators[i].activation_eligibility_epoch == if is_eligible_for_activation_queue(s.validators[i]) then get_current_epoch(s) + 1 
-    //     //                                                             else s.validators[i].activation_eligibility_epoch;
-    //     //     // i.e. even if made eligible for the activation queue, these validators won't be active validators and so don't overlap with the next section
-            
-    //     //     //assert get_current_epoch(s) < FAR_FUTURE_EPOCH;
-            
-    //     //     // is_active_validator: validator.activation_epoch <= epoch < validator.exitEpoch
-    //     //     if is_active_validator(s.validators[i],  get_current_epoch(s)) && s.validators[i].effective_balance <= EJECTION_BALANCE {
-    //     //         // initiate_validator_exit(state, ValidatorIndex(index))
-    //     //         assert !(is_eligible_for_activation_queue(s.validators[i]) && s'.validators[i].effective_balance <= EJECTION_BALANCE);
-    //     //         assert s'.validators[i] == s.validators[i];
-    //     //         s' := initiate_validator_exit(s', i as ValidatorIndex);   
-    //     //     }
-    //     // //    assert s'.validators[i].exitEpoch == if is_active_validator(s.validators[i],  get_current_epoch(s)) && s.validators[i].effective_balance <= EJECTION_BALANCE
-    //     // //                                 then initiate_validator_exit(s', i as ValidatorIndex).validators[i].exitEpoch
-    //     // //                                 else s.validators[i].exitEpoch;
-            
-            
-    //     //     i := i  + 1;
-    //     //     //assert s' == updateEligibilityAndEjectionsHelper(s', i);
-    //     // }
-
-
-
-    //     //     # Queue validators eligible for activation and not yet dequeued for activation
-    //     //     activation_queue = sorted([
-    //     //     index for index, validator in enumerate(state.validators)
-    //     //     if is_eligible_for_activation(state, validator)
-    //     //     # Order by the sequence of activation_eligibility_epoch setting and then index
-    //     //     ], key=lambda index: (state.validators[index].activation_eligibility_epoch, index))
-    //     var activation_queue := get_activation_queue(s', 0);
-    //     // @Note: in a simplification of the spec the activiation queue is not sorted
-
-
-    //     var k := 0;
-
-    //     //assert s' == updateRegistry(s); // need to functional equivalents??
-
-    //     // # Dequeued validators for activation up to churn limit
-    //     // for index in activation_queue[:get_validator_churn_limit(state)]:
-    //     //     validator = state.validators[index]
-    //     //     validator.activation_epoch = compute_activation_exit_epoch(get_current_epoch(state))
-    //     // var churn_limit := get_validator_churn_limit(s') ;
-    //     // assume churn_limit as nat <= |activation_queue| <= |s'.validators|;
-    //     // assume forall index :: 0 <= index < |activation_queue[..churn_limit]| ==> activation_queue[index] as nat < |s'.validators|;
-        
-    //     // while j < |activation_queue[..churn_limit]|
-    //     //     invariant  |s.validators| == |s.balances| ==|s'.balances| == |s'.validators|
-    //     //     invariant j <= |s'.validators| == |s'.balances| 
-    //     //     // invariant forall v :: i <= v < |s.balances| ==> s'.balances[v] ==  s.balances[v]
-            
-    //     //     // invariant s' == s.(validators := s'.validators)
-    //     // {
-    //     //     assert activation_queue[j] as nat < |s'.validators|;
-    //     //     s' := s'.(validators := s'.validators[activation_queue[j] := s'.validators[activation_queue[j]].(activation_epoch := compute_activation_exit_epoch(get_current_epoch(s')))]);   
-    //     //     j := j  + 1;
-    //     // }
-    // }
-
-    // // // lemma RegistryHelperLemma(s: BeaconState, i: ValidatorIndex)
-    // // //     requires get_current_epoch(s) < FAR_FUTURE_EPOCH
-    // // //     requires i as nat < |s.validators|
-    // // //     ensures !(is_eligible_for_activation_queue(s.validators[i]) && s.validators[i].effective_balance <= EJECTION_BALANCE)
-    // // // {
-    // // //     assert is_eligible_for_activation_queue(s.validators[i]) ==> s.validators[i].effective_balance == MAX_EFFECTIVE_BALANCE;
-
-    // // // }
-    
-
+    /** 
+     *  Process slashings.
+     *  
+     *  @param  s   A state.
+     *  @returns    The state obtained after applying the epoch slashings.
+     *
+     *  @note       This function uses assume statements as a simplification to ensure
+     *              that balance overflows don't occur. To remove these assume statements
+     *              a strategy similar to that applied within the deposit processing
+     *              could be applied.
+     */
     method process_slashings(s: BeaconState) returns (s' : BeaconState)
         requires |s.validators| == |s.balances| 
+
         ensures |s'.validators| == |s'.balances| 
         ensures s' == updateSlashings(s)
     {
         var epoch := get_current_epoch(s);
         var total_balance := get_total_active_balance_full(s);
         var sumSlashings := get_total_slashings(s.slashings);
-        var adjusted_total_slashing_balance := min((sumSlashings as nat * PROPORTIONAL_SLASHING_MULTIPLIER as nat) as nat, total_balance as nat) as Gwei;
-        var increment := EFFECTIVE_BALANCE_INCREMENT;  // Factored out from penalty numerator to avoid uint64 overflow
+        var adjusted_total_slashing_balance := 
+            min((sumSlashings as nat * PROPORTIONAL_SLASHING_MULTIPLIER as nat) as nat, 
+                total_balance as nat) as Gwei;
+        var increment := EFFECTIVE_BALANCE_INCREMENT;  
+        // Factored out from penalty numerator to avoid uint64 overflow
         
         assert total_balance > 0 as Gwei;
         assert increment > 0 as Gwei;
-        assume forall v :: 0 <= v < |s.validators| ==> 0 <= s.validators[v].effective_balance as nat * adjusted_total_slashing_balance as nat / total_balance  as nat < 0x10000000000000000;
-        assume epoch as nat + EPOCHS_PER_SLASHINGS_VECTOR as nat / 2 < 0x10000000000000000;
-            
-    
+        assume forall v :: 0 <= v < |s.validators| 
+                ==> 0 
+                <= s.validators[v].effective_balance as nat * adjusted_total_slashing_balance as nat / total_balance  as nat 
+                < 0x10000000000000000;
+        assume epoch as nat + EPOCHS_PER_SLASHINGS_VECTOR as nat / 2 
+                < 0x10000000000000000;
+
         s' := s;
         var i := 0;
-        assert s' == updateSlashingsHelper(s, i, epoch, total_balance, adjusted_total_slashing_balance, increment);
+        assert s' == updateSlashingsHelper(s, 
+                                           i, 
+                                           epoch, 
+                                           total_balance, 
+                                           adjusted_total_slashing_balance, 
+                                           increment);
 
         while i < |s'.balances|
             invariant  |s.validators| == |s.balances| ==|s'.balances| == |s'.validators|
             invariant i <= |s'.validators| == |s'.balances| 
             invariant s.validators == s'.validators
             invariant forall v :: i <= v < |s.balances| ==> s'.balances[v] ==  s.balances[v]
-
-            //ensures |s'.validators| == |s.validators| 
-            //ensures |s'.balances| == |s.balances| 
-        
-            //ensures forall v :: 0 <= v < |s.validators| ==> s'.validators[v]  == s.validators[v]
             invariant s' == s.(balances := s'.balances)
-            //ensures forall v :: len <= v < |s.balances| ==> s'.balances[v]  == s.balances[v]
-
-
             invariant s' == s.(balances := s'.balances)
-            
             invariant forall v :: 0 <= v < i ==> 
-        
                 assert v < |s.balances|;
-
-                var new_bal := if (s.validators[v].slashed && (epoch + EPOCHS_PER_SLASHINGS_VECTOR / 2) == s.validators[v].withdrawable_epoch)
-                                        // then if s.balances[v] > penalty as Gwei then s.balances[v] - penalty as Gwei
-                                        //                                                 else 0 as Gwei
-                                        then decrease_balance(s, v as ValidatorIndex, (s.validators[v].effective_balance as nat * adjusted_total_slashing_balance as nat / total_balance  as nat) as Gwei).balances[v]
-                                        else s.balances[v];
-                updateSlashingsHelper(s, i, epoch, total_balance, adjusted_total_slashing_balance, increment).balances[v] == new_bal
+                var new_bal := if (s.validators[v].slashed && (epoch + EPOCHS_PER_SLASHINGS_VECTOR / 2) 
+                                    == s.validators[v].withdrawable_epoch)
+                                    then decrease_balance(s, 
+                                                          v as ValidatorIndex, 
+                                                          (s.validators[v].effective_balance as nat * adjusted_total_slashing_balance as nat / total_balance as nat) as Gwei
+                                                         ).balances[v]
+                                    else s.balances[v];
+                updateSlashingsHelper(s, 
+                                      i, 
+                                      epoch, 
+                                      total_balance, 
+                                      adjusted_total_slashing_balance, increment
+                                     ).balances[v] == new_bal
             invariant s' == updateSlashingsHelper(s, i, epoch, total_balance, adjusted_total_slashing_balance, increment)
-            
         {
-            // var penalty_numerator := s'.validators[i].effective_balance as nat / increment as nat * adjusted_total_slashing_balance as nat;
-            // var penalty := penalty_numerator as nat / total_balance  as nat * increment as nat;
-            // assume 0 <= penalty < 0x10000000000000000;
-            
             if (s'.validators[i].slashed && (epoch + EPOCHS_PER_SLASHINGS_VECTOR / 2) == s'.validators[i].withdrawable_epoch) {
-                
-                s' := decrease_balance(s', i as ValidatorIndex, (s.validators[i].effective_balance as nat * adjusted_total_slashing_balance as nat / total_balance  as nat) as Gwei);
+                s' := decrease_balance(s', 
+                                       i as ValidatorIndex, 
+                                       (s.validators[i].effective_balance as nat * adjusted_total_slashing_balance as nat / total_balance  as nat) as Gwei);
             }
-    
-            //assert s.validators == s'.validators;
-            assert s'.balances[i] == if (s.validators[i].slashed && (epoch + EPOCHS_PER_SLASHINGS_VECTOR / 2) == s.validators[i].withdrawable_epoch)
-                                            // then 
-                                            //     if s.balances[i] > penalty as Gwei then s.balances[i] - penalty as Gwei
-                                            //                                         else 0 as Gwei
-                                            then decrease_balance(s, i as ValidatorIndex, (s.validators[i].effective_balance as nat * adjusted_total_slashing_balance as nat / total_balance  as nat) as Gwei).balances[i]
-                                            else s.balances[i];
-            //assert forall v :: i < v < |s.balances| ==> s'.balances[v] == s.balances[v];
+            
+            assert s'.balances[i] == if (s.validators[i].slashed && (epoch + EPOCHS_PER_SLASHINGS_VECTOR / 2) 
+                                        == s.validators[i].withdrawable_epoch)
+                                        then decrease_balance(s, 
+                                                              i as ValidatorIndex, 
+                                                              (s.validators[i].effective_balance as nat * adjusted_total_slashing_balance as nat / total_balance as nat) as Gwei
+                                                             ).balances[i]
+                                        else s.balances[i];
             i := i + 1;
-            // assert i <= |s.balances| == |s.validators| ;
-            // assert total_balance > 0 as Gwei;
-            // assert increment > 0 as Gwei;
-            // assert forall v :: 0 <= v < |s.validators| ==> 0 <= s.validators[v].effective_balance as nat * adjusted_total_slashing_balance as nat / total_balance  as nat < 0x10000000000000000;
-            // assert epoch as nat + EPOCHS_PER_SLASHINGS_VECTOR as nat / 2 < 0x10000000000000000;
-            // assert s' == updateSlashingsHelper(s, i, epoch, total_balance, adjusted_total_slashing_balance, increment);
-        
         }
-        //assert |s.balances| == |s.validators|;
-
         assert s' == updateSlashingsHelper(s, i, epoch, total_balance, adjusted_total_slashing_balance, increment);
         assert i == |s'.validators|;
         assert s' == updateSlashings(s);
     }
 
-    
-
-    
-
-
+    /** 
+     *  Process eth1 data reset.
+     *  
+     *  @param  s   A state.
+     *  @returns    The state obtained after applying the epoch eth1 data reset.
+     */
     method process_eth1_data_reset(s: BeaconState) returns (s' : BeaconState)
         ensures s' == updateEth1DataReset(s)
     {
@@ -532,185 +371,26 @@ module EpochProcessing {
         else {s' := s;}
     }
     
-
+    /** 
+     *  Process effective balance updates.
+     *  
+     *  @param  s   A state.
+     *  @returns    The state obtained after applying the epoch effective balance updates
+     *
+     *  @note       This component has been simplified.
+     */
     method process_effective_balance_updates(s: BeaconState) returns (s' : BeaconState)
-        requires |s.balances| == |s.validators|
         ensures s' == updateEffectiveBalance(s)
     {
         s' := s;
-        
-        var i := 0;
-        assert s' == updateEffectiveBalanceHelper(s, i);
-        //assume forall v :: 0 <= v < |rewards| ==> s.balances[v] as nat + rewards[v] as nat < 0x10000000000000000;
-        var HYSTERESIS_INCREMENT := EFFECTIVE_BALANCE_INCREMENT / HYSTERESIS_QUOTIENT;
-        var DOWNWARD_THRESHOLD := HYSTERESIS_INCREMENT * HYSTERESIS_DOWNWARD_MULTIPLIER;
-        var UPWARD_THRESHOLD := HYSTERESIS_INCREMENT * HYSTERESIS_UPWARD_MULTIPLIER;
-
-        assume forall v :: i <= v < |s.validators| ==> s.balances[v] as nat + DOWNWARD_THRESHOLD as nat  < 0x10000000000000000;
-        assume forall v :: i <= v < |s.validators| ==> s.validators[v].effective_balance as nat + UPWARD_THRESHOLD as nat  < 0x10000000000000000;
-        assert forall v :: i <= v < |s.validators| ==> 0 <= (s.balances[v] % EFFECTIVE_BALANCE_INCREMENT) < EFFECTIVE_BALANCE_INCREMENT;
-        assert forall v :: i <= v < |s.validators| ==> s.balances[v] >= (s.balances[v] % EFFECTIVE_BALANCE_INCREMENT);
-        
-        while i < |s'.balances| //for index in range(len(state.validators)):
-            invariant  |s.validators| == |s.balances| ==|s'.balances| == |s'.validators|
-            invariant i <= |s'.validators|
-            invariant forall v :: i <= v < |s.validators| ==> s'.validators[v]  == s.validators[v];
-            invariant s' == s.(validators := s'.validators);
-            
-            invariant s'.balances == s.balances
-            invariant forall v :: i <= v < |s.validators| ==> s'.validators[v].effective_balance ==  s.validators[v].effective_balance;
-            invariant forall v :: i <= v < |s.balances| ==> s'.balances[v] ==  s.balances[v];
-            // invariant forall v :: 0 <= v < i ==> 
-            //                 s'.validators[v].effective_balance ==  
-            //                         if (s.balances[v]+ DOWNWARD_THRESHOLD < s.validators[v].effective_balance || s.validators[v].effective_balance + UPWARD_THRESHOLD < s.balances[v]) 
-            //                             then min((s.balances[v] - (s.balances[v] % EFFECTIVE_BALANCE_INCREMENT)) as nat, MAX_EFFECTIVE_BALANCE as nat) as Gwei 
-            //                             else s.validators[v].effective_balance;
-
-            invariant forall v :: 0 <= v < i ==> 
-                    var balance := s.balances[v];
-                    var HYSTERESIS_INCREMENT := EFFECTIVE_BALANCE_INCREMENT / HYSTERESIS_QUOTIENT;
-                    var DOWNWARD_THRESHOLD := HYSTERESIS_INCREMENT * HYSTERESIS_DOWNWARD_MULTIPLIER;
-                    var UPWARD_THRESHOLD := HYSTERESIS_INCREMENT * HYSTERESIS_UPWARD_MULTIPLIER;
-                    assume balance as nat + DOWNWARD_THRESHOLD as nat  < 0x10000000000000000;
-                    assume s.validators[v].effective_balance as nat + UPWARD_THRESHOLD as nat  < 0x10000000000000000;
-                    assert 0 <= (balance % EFFECTIVE_BALANCE_INCREMENT) < EFFECTIVE_BALANCE_INCREMENT;
-                    assert balance >= (balance % EFFECTIVE_BALANCE_INCREMENT);
-                    //assert balance - (balance % EFFECTIVE_BALANCE_INCREMENT) >= 0;
-
-                    // s'.validators[v].effective_balance ==  
-                    //                     if (balance + DOWNWARD_THRESHOLD < s.validators[v].effective_balance || s.validators[v].effective_balance + UPWARD_THRESHOLD < balance) 
-                    //                         then min((balance - (balance % EFFECTIVE_BALANCE_INCREMENT)) as nat, MAX_EFFECTIVE_BALANCE as nat) as Gwei 
-                    //                         else s.validators[v].effective_balance;
-                    var new_bal := if (s.balances[v] + DOWNWARD_THRESHOLD < s.validators[v].effective_balance || s.validators[v].effective_balance + UPWARD_THRESHOLD < s.balances[v]) 
-                                        then min((s.balances[v] - (s.balances[v] % EFFECTIVE_BALANCE_INCREMENT)) as nat, MAX_EFFECTIVE_BALANCE as nat) as Gwei 
-                                        else s.validators[v].effective_balance;
-                    s'.validators[v] == s.validators[v].(effective_balance := new_bal);
-            
-           //invariant s' == updateEffectiveBalanceHelper(s, i)
-        {
-            var balance := s'.balances[i];
-            if (balance + DOWNWARD_THRESHOLD < s'.validators[i].effective_balance || s'.validators[i].effective_balance + UPWARD_THRESHOLD < balance) {
-                    s' := s'.(validators := s'.validators[i := s'.validators[i].(effective_balance := min((balance - (balance % EFFECTIVE_BALANCE_INCREMENT)) as nat, MAX_EFFECTIVE_BALANCE as nat) as Gwei)]);
-                }
-            
-            assert s'.validators[i].effective_balance == if (balance + DOWNWARD_THRESHOLD < s.validators[i].effective_balance || s.validators[i].effective_balance + UPWARD_THRESHOLD < balance) 
-                                                         then min((balance - (balance % EFFECTIVE_BALANCE_INCREMENT)) as nat, MAX_EFFECTIVE_BALANCE as nat) as Gwei 
-                                                         else s.validators[i].effective_balance;
-            
-            assert  i <= |s.balances| == |s.validators|;
-            assert |s'.validators| == |s.validators|;
-            assert |s'.balances| == |s.balances|;
-            assert s'.balances == s.balances;
-            //requires forall v :: i <= v < |s.validators| ==> s'.validators[v].effective_balance  == s.validators[v].effective_balance
-            
-            // assert forall v :: 0 <= v < i ==> 
-            //         var balance := s.balances[v];
-            //         var HYSTERESIS_INCREMENT := EFFECTIVE_BALANCE_INCREMENT / HYSTERESIS_QUOTIENT;
-            //         var DOWNWARD_THRESHOLD := HYSTERESIS_INCREMENT * HYSTERESIS_DOWNWARD_MULTIPLIER;
-            //         var UPWARD_THRESHOLD := HYSTERESIS_INCREMENT * HYSTERESIS_UPWARD_MULTIPLIER;
-            //         assume balance as nat + DOWNWARD_THRESHOLD as nat  < 0x10000000000000000;
-            //         assume s.validators[v].effective_balance as nat + UPWARD_THRESHOLD as nat  < 0x10000000000000000;
-            //         assert 0 <= (balance % EFFECTIVE_BALANCE_INCREMENT) < EFFECTIVE_BALANCE_INCREMENT;
-            //         assert balance >= (balance % EFFECTIVE_BALANCE_INCREMENT);
-            //         //assert balance - (balance % EFFECTIVE_BALANCE_INCREMENT) >= 0;
-
-            //         // s'.validators[v].effective_balance ==  
-            //         //                     if (balance + DOWNWARD_THRESHOLD < s.validators[v].effective_balance || s.validators[v].effective_balance + UPWARD_THRESHOLD < balance) 
-            //         //                         then min((balance - (balance % EFFECTIVE_BALANCE_INCREMENT)) as nat, MAX_EFFECTIVE_BALANCE as nat) as Gwei 
-            //         //                         else s.validators[v].effective_balance;
-            //         var new_bal := if (s.balances[v] + DOWNWARD_THRESHOLD < s.validators[v].effective_balance || s.validators[v].effective_balance + UPWARD_THRESHOLD < s.balances[v]) 
-            //                             then min((s.balances[v] - (s.balances[v] % EFFECTIVE_BALANCE_INCREMENT)) as nat, MAX_EFFECTIVE_BALANCE as nat) as Gwei 
-            //                             else s.validators[v].effective_balance;
-            //         s'.validators[v] == s.validators[v].(effective_balance := new_bal);
-                
-                
-            
-            i := i +1;
-            //hope1(s, s', i);
-            assert s' == updateEffectiveBalanceHelper(s, i);
-        }
-        
-        //hope1(s, s', i);
-        assert |s.balances| == |s.validators|;
-        //assert |s'.validators| == |s.validators|;
-        //assert |s'.balances| == |s.balances|;
-        //assert s'.balances == s.balances;
-
-        assert s' == updateEffectiveBalanceHelper(s, i);
-        assert i == |s'.validators|;
-        assert s' == updateEffectiveBalance(s);
     }
-
-    // lemma hope1(s: BeaconState, s': BeaconState, i: nat)
-    //     requires  i <= |s.balances| == |s.validators|
-    //     requires |s'.validators| == |s.validators|
-    //     requires |s'.balances| == |s.balances|
-    //     requires s'.balances == s.balances
-    //     //requires forall v :: i <= v < |s.validators| ==> s'.validators[v].effective_balance  == s.validators[v].effective_balance
-    //     requires s' == s.(validators := s'.validators)
-    //     requires forall v :: i <= v < |s.validators| ==> s'.validators[v]  == s.validators[v]
-        
-    //     requires forall v :: 0 <= v < i ==> 
-    //             var balance := s.balances[v];
-    //             var HYSTERESIS_INCREMENT := EFFECTIVE_BALANCE_INCREMENT / HYSTERESIS_QUOTIENT;
-    //             var DOWNWARD_THRESHOLD := HYSTERESIS_INCREMENT * HYSTERESIS_DOWNWARD_MULTIPLIER;
-    //             var UPWARD_THRESHOLD := HYSTERESIS_INCREMENT * HYSTERESIS_UPWARD_MULTIPLIER;
-    //             assume balance as nat + DOWNWARD_THRESHOLD as nat  < 0x10000000000000000;
-    //             assume s.validators[v].effective_balance as nat + UPWARD_THRESHOLD as nat  < 0x10000000000000000;
-    //             assert 0 <= (balance % EFFECTIVE_BALANCE_INCREMENT) < EFFECTIVE_BALANCE_INCREMENT;
-    //             assert balance >= (balance % EFFECTIVE_BALANCE_INCREMENT);
-    //             //assert balance - (balance % EFFECTIVE_BALANCE_INCREMENT) >= 0;
-
-    //             // s'.validators[v].effective_balance ==  
-    //             //                     if (balance + DOWNWARD_THRESHOLD < s.validators[v].effective_balance || s.validators[v].effective_balance + UPWARD_THRESHOLD < balance) 
-    //             //                         then min((balance - (balance % EFFECTIVE_BALANCE_INCREMENT)) as nat, MAX_EFFECTIVE_BALANCE as nat) as Gwei 
-    //             //                         else s.validators[v].effective_balance;
-    //             var new_bal := if (s.balances[v] + DOWNWARD_THRESHOLD < s.validators[v].effective_balance || s.validators[v].effective_balance + UPWARD_THRESHOLD < s.balances[v]) 
-    //                                 then min((s.balances[v] - (s.balances[v] % EFFECTIVE_BALANCE_INCREMENT)) as nat, MAX_EFFECTIVE_BALANCE as nat) as Gwei 
-    //                                 else s.validators[v].effective_balance;
-    //             s'.validators[v] == s.validators[v].(effective_balance := new_bal);
-            
-    //             //s'.validators[v].pubkey == s.validators[v].pubkey &&
-    //             //s'.validators[v].effective_balance == new_bal &&
-    //             //s'.validators[v].slashed == s.validators[v].slashed &&
-    //             //s'.validators[v].activationEpoch == s.validators[v].activationEpoch &&
-    //             //s'.validators[v].exitEpoch == s.validators[v].exitEpoch &&
-    //             //s'.validators[v].withdrawable_epoch == s.validators[v].withdrawable_epoch 
-    //     ensures  s' == updateEffectiveBalanceHelper(s, i)
-    // {
-    //     // Thanks Dafny
-    //     assert s'.balances == updateEffectiveBalanceHelper(s, i).balances;
-    //     assert forall v :: i <= v < |s.validators| ==> s'.validators[v] == updateEffectiveBalanceHelper(s, i).validators[v];
-    //     assert forall v :: 0 <= v < i ==> 
-    //         // var balance := s.balances[v];
-    //         var HYSTERESIS_INCREMENT := EFFECTIVE_BALANCE_INCREMENT / HYSTERESIS_QUOTIENT;
-    //         var DOWNWARD_THRESHOLD := HYSTERESIS_INCREMENT * HYSTERESIS_DOWNWARD_MULTIPLIER;
-    //         var UPWARD_THRESHOLD := HYSTERESIS_INCREMENT * HYSTERESIS_UPWARD_MULTIPLIER;
-
-    //         assume s.balances[v] as nat + DOWNWARD_THRESHOLD as nat  < 0x10000000000000000;
-    //         assume s.validators[v].effective_balance as nat + UPWARD_THRESHOLD as nat  < 0x10000000000000000;
-
-    //         //updateEffectiveBalanceHelper(s, len).validators[v].effective_balance == 
-    //         var new_bal := if (s.balances[v] + DOWNWARD_THRESHOLD < s.validators[v].effective_balance || s.validators[v].effective_balance + UPWARD_THRESHOLD < s.balances[v]) 
-    //                                 then min((s.balances[v] - (s.balances[v] % EFFECTIVE_BALANCE_INCREMENT)) as nat, MAX_EFFECTIVE_BALANCE as nat) as Gwei 
-    //                                 else s.validators[v].effective_balance;
-    //         updateEffectiveBalanceHelper(s, i).validators[v] == s.validators[v].(effective_balance := new_bal);
-    //         //updateEffectiveBalanceHelper(s, i).validators[v].pubkey == s'.validators[v].pubkey &&
-    //         //updateEffectiveBalanceHelper(s, i).validators[v].effective_balance == new_bal == s'.validators[v].effective_balance &&
-    //         //updateEffectiveBalanceHelper(s, i).validators[v].slashed == s'.validators[v].slashed &&
-    //         //updateEffectiveBalanceHelper(s, i).validators[v].activationEpoch == s'.validators[v].activationEpoch &&
-    //         //updateEffectiveBalanceHelper(s, i).validators[v].exitEpoch == s'.validators[v].exitEpoch &&
-    //         //updateEffectiveBalanceHelper(s, i).validators[v].withdrawable_epoch == s'.validators[v].withdrawable_epoch ;
-    //     assert  s' == updateEffectiveBalanceHelper(s, i);
-    // }
-
-
-
     
-
-    
-    
-    /**/
+    /** 
+     *  Process slashings reset.
+     *  
+     *  @param  s   A state.
+     *  @returns    The state obtained after applying the epoch slashings reset.
+     */
     method process_slashings_reset(s: BeaconState) returns (s' : BeaconState)
         ensures s' == updateSlashingsReset(s)
     {
@@ -719,26 +399,32 @@ module EpochProcessing {
         s' := s.(
                 slashings := s.slashings[(next_epoch % EPOCHS_PER_SLASHINGS_VECTOR) as nat := 0 as Gwei]
             );
-
     }
 
-
-    /**/
+    /** 
+     *  Process randao mixes reset.
+     *  
+     *  @param  s   A state.
+     *  @returns    The state obtained after applying the epoch randao mixes reset.
+     */
     method process_randao_mixes_reset(s: BeaconState) returns (s' : BeaconState)
         ensures s' == updateRandaoMixes(s)
     {
         var current_epoch := get_current_epoch(s);
         var next_epoch := current_epoch + 1;
-        // Set randao mix
-        // state.randao_mixes[next_epoch % EPOCHS_PER_HISTORICAL_VECTOR] = get_randao_mix(s, current_epoch)
         s' := s.(
-                randao_mixes := s.randao_mixes[(next_epoch % EPOCHS_PER_HISTORICAL_VECTOR) as nat := get_randao_mix(s, current_epoch)]
+                randao_mixes := s.randao_mixes[
+                            (next_epoch % EPOCHS_PER_HISTORICAL_VECTOR) as nat := get_randao_mix(s, current_epoch)
+                        ]
             );
-
     }
     
-    
-    /**/
+    /** 
+     *  Process the historical roots update.
+     *  
+     *  @param  s   A state.
+     *  @returns    The state obtained after applying the epoch historical roots update.
+     */
     method process_historical_roots_update(s: BeaconState) returns (s' : BeaconState)
         ensures s' == updateHistoricalRoots(s)
     {
@@ -756,10 +442,7 @@ module EpochProcessing {
     /**
      *  Rotate the attestations.
      *  @param  s   A state.
-     *  @returns    `s` with attestations rotated.
-     *
-     *  @todo       This is a partial implementation capturing only
-     *              the attestations updates.
+     *  @return    `s` with attestations rotated.
      */
     method process_participation_record_updates(s: BeaconState) returns (s' : BeaconState)
         ensures s' == updateParticipationRecords(s)
